@prefix : <https://w3id.org/abdn/foodsafety/fs-prov#> .
@prefix owl: <http://www.w3.org/2002/07/owl#> .
@prefix rdf: <http://www.w3.org/1999/02/22-rdf-syntax-ns#> .
@prefix xml: <http://www.w3.org/XML/1998/namespace> .
@prefix xsd: <http://www.w3.org/2001/XMLSchema#> .
@prefix rdfs: <http://www.w3.org/2000/01/rdf-schema#> .
@base <https://w3id.org/abdn/foodsafety/fs-prov> .

<https://w3id.org/abdn/foodsafety/fs-prov> rdf:type owl:Ontology .


#################################################################
#
#    Object Properties
#
#################################################################


###  https://w3id.org/abdn/foodsafety/fs-prov#entity

:entity rdf:type owl:ObjectProperty ;
        
        rdfs:domain owl:Thing ;
        
        rdfs:comment """ 
        A relation that links the instantiation of some fs-prov:Resource to an sc-prov:EvaluationContext. 
        The fs-prov:Resource should be restricted by an fs-prov:Constraint which is also linked to the same sc-prov:EvaluationContext
        """ ;
        
        rdfs:range :WorkflowEntity .



###  https://w3id.org/abdn/foodsafety/fs-prov#hasGoal

:hasGoal rdf:type owl:ObjectProperty ;
         
         rdfs:domain :Plan ;
         
         rdfs:comment """ 
         A relation that links an instance of a plan to the final expected product denoted as an fs-prov:Resource.
         """ ;
         
         rdfs:range :Resource .



###  https://w3id.org/abdn/foodsafety/fs-prov#hasParameter

:hasConstraintParameter rdf:type owl:ObjectProperty ;

        rdfs:comment """ 
        An fs-prov:hasConstraintParameter links instantiations of  fs-prov: Parameter as a source of parameter values  for an fs-prov:Constraint.
        """ ;
              
        rdfs:domain :Constraint ;
              
        rdfs:range :Parameter .



###  https://w3id.org/abdn/foodsafety/fs-prov#inContextOf

:inContextOf rdf:type owl:ObjectProperty ;

        rdfs:comment """ 
        A property that defines which fs-prov:Resource is associated with a property described as an fs-prov:Parameter.
        """ ;
         
         rdfs:domain :Parameter ;
             
         rdfs:range :Resource .



###  https://w3id.org/abdn/foodsafety/fs-prov#instantiatedByActivity

:instantiatedByActivity rdf:type owl:ObjectProperty ;
                        
        rdfs:domain :Step ;
        
        rdfs:comment """ 
        A property that links an fs-prov:Step to its instantiation in  a workflow execution described by a prov:Activity. 
        """ ;
                        
        rdfs:range :WorkflowActivity .



###  https://w3id.org/abdn/foodsafety/fs-prov#instantiatedByEntity

:instantiatedByEntity rdf:type owl:ObjectProperty ;
                      
        rdfs:comment """ 
        A property that links an fs-prov:Resource to its instantiation in  a workflow execution described by a prov:Entity. 
        """ ;
                      
        rdfs:domain :Resource ;
                      
        rdfs:range :WorkflowEntity .



###  https://w3id.org/abdn/foodsafety/fs-prov#isOptionalResourceFor

:isOptionalResourceFor rdf:type owl:ObjectProperty ;
               
        rdfs:comment """ 
         A property that links an fs-prov:Step to an fs-prov: Resource which could  be used by the instantiation of this step. 
        """ ;
           
             
        rdfs:domain :Resource ;
                       
        rdfs:range :Step .



###  https://w3id.org/abdn/foodsafety/fs-prov#isRequiredResourceFor

:isRequiredResourceFor rdf:type owl:ObjectProperty ;

        rdfs:comment """ 
        A property that links an fs-prov:Step to an fs-prov: Resource which has to be used by the instantiation of this step. 
        """ ;
                       
        rdfs:domain :Resource ;
                       
        rdfs:range :Step .



###  https://w3id.org/abdn/foodsafety/fs-prov#isResultOf

        rdfs:comment """ 
        A property that links an fs-prov:Step to its expected product described as fs-prov: Resource.  
        """ ;

        :isResultOf rdf:type owl:ObjectProperty ;
        
        rdfs:domain :Resource ;
                       
        rdfs:range :Step .



###  https://w3id.org/abdn/foodsafety/fs-prov#restrics

:restrics rdf:type owl:ObjectProperty ;

        rdfs:comment """ 
        A property that associates restrictions identified by an fs-prov:Constraint with a specific fs-prov:Resource. 
        """ ;
          
          rdfs:domain :Constraint ;
          
          rdfs:range :Resource .





#################################################################
#
#    Classes
#
#################################################################


###  https://w3id.org/abdn/foodsafety/fs-prov#Constraint

:Constraint rdf:type owl:Class ;

        rdfs:comment """ 
        An fs-prov: Constraint identifies a logical statement that describes some restrictions on fs-prov:Resource in the context of an fs-prov:Step. 
        """ .



###  https://w3id.org/abdn/foodsafety/fs-prov#HaccpConstraint

:HaccpConstraint rdf:type owl:Class ;
                 
                 rdfs:subClassOf :Constraint ;
                 
                 rdfs:comment """ 
                An fs-prov: HACCPConstraint identifies a logical statement that describes some restrictions on an 
                fs-prov:Resource in the context of an fs-prov:HACCPStep. fs-prov: HACCPConstraint is typically defined 
                in the context of maximum or minimum threshold values of some properties relating to an fs-prov:Resource
                """ .



###  https://w3id.org/abdn/foodsafety/fs-prov#HaccpStep

:HaccpStep rdf:type owl:Class ;
           
           rdfs:subClassOf :Step ;
           
           rdfs:comment """ 
           An fs-prov: HACCPStep denotes parts of a workflow plan which represent expected HACCP-regulated activities 
           that transform fs-prov: PhysicalObject(s).
           """ .



###  https://w3id.org/abdn/foodsafety/fs-prov#Parameter

:Parameter rdf:type owl:Class ;
           
           rdfs:subClassOf :Resource ;
           
           rdfs:comment """ 
           An fs-prov: Parameter denotes parts of a workflow plan, which can be used by an fs-prov:Constraint 
           to determine variables of a restriction defined by fs-prov:Constraint. 
           """ .



###  https://w3id.org/abdn/foodsafety/fs-prov#PhysicalObject

:PhysicalObject rdf:type owl:Class ;
                
                rdfs:subClassOf :Resource ;
                
                rdfs:comment """ 
                An fs-prov: PhysicalObject represents a certain type of non-virtual entity that can be used or produced by an fs-prov:Step.
                """ .



###  https://w3id.org/abdn/foodsafety/fs-prov#Plan

:Plan rdf:type owl:Class ;

rdfs:comment """ 
An fs-prov:Plan is a specific type of p-plan:Plan. It is composed of fs-prov:Step(s), fs-prov:Resource(s) and fs-prov:Constraint(s). 
Individual concept mentions are expected to represent a specific part of a single unique plan.  
Hence, URIâ€™s of these concepts are not to be reused in other plans or even within the same plan. 
""" .



###  https://w3id.org/abdn/foodsafety/fs-prov#Resource

:Resource rdf:type owl:Class ;

rdfs:comment """ 
An fs-prov: Resource denotes parts of a workflow plan, which can be used by an 
fs-prov:Step and fs-prov:Constraint or produced by an fs-prov:Step.  
""" .



###  https://w3id.org/abdn/foodsafety/fs-prov#Step

:Step rdf:type owl:Class ;

rdfs:comment """ 
An fs-prov: Step denotes parts of a workflow plan which represent expected activities that transform fs-prov: Resource(s).  
""" .



###  https://w3id.org/abdn/foodsafety/fs-prov#WorkflowActivity

:WorkflowActivity rdf:type owl:Class ;

rdfs:comment """ 
An fs-prov: WorkflowActivity is a subclass of prov:Activity and represents an instantiation of fs-prov:Step during a workflow execution.   
""" .



###  https://w3id.org/abdn/foodsafety/fs-prov#WorkflowEntity

:WorkflowEntity rdf:type owl:Class ;

rdfs:comment """ 
An fs-prov: WorkflowEntity is a subclass of prov:Entity and represents an instantiation of fs-prov:Resorce during a workflow execution.  
""" .




###  Generated by the OWL API (version 3.5.1) http://owlapi.sourceforge.net
